x86model/Model/Vector.v
@@ -1,0 +1,16 @@
+Require Import List.
+Axiom vector : Type -> Type.
+Axiom length : forall {A}, vector A -> nat.
+Axiom get : forall {A} (v:vector A) (i:nat), (i < length v) -> A.
+Axiom of_list : forall {A}, list A -> vector A.
+
+Axiom get_of_list : 
+  forall A (l:list A) i (H:i < length (of_list l)), 
+    nth_error l i = Some (@get _ (of_list l) i H).
+Axiom length_of_list : 
+  forall A (l:list A), length (of_list l) = List.length l.
+
+Extract Constant vector "'a" => "'a array".
+Extract Constant length => "fun v => Big.of_int (Array.length v)".
+Extract Constant get => "fun v i => Array.get v (Big.to_int i)".
+Extract Inlined Constant of_list => "Array.of_list".
